theories/LambdaANF/toplevel.v
@@ -9,6 +9,9 @@ From CertiCoq Require Import LambdaBoxLocal.toplevel.
 
 Require Import Common.Common Common.compM Common.Pipeline_utils.
 Require Import ExtLib.Structures.Monad.
+Require Import MetaCoq.Utils.bytestring.
+Require Import MetaCoq.Template.All.
+(* From MetaCoq.Template Require Import Kernames.string_of_kername. *)
 
 Import Monads.
 
@@ -191,7 +194,7 @@ Section IDENT.
       e <- (if inl_known anf_opts then
               time_anf "Inline known functions inside wrappers" (inline_lifted next_var 10 1000) e
             else id_trans e) ;;
-      ret e. 
+      ret e.
 
 
     Definition run_anf_pipeline (t : LambdaANF_FullTerm) : error LambdaANF_FullTerm * string :=
@@ -209,8 +212,10 @@ Section IDENT.
         (Err ("Failed compiling LambdaANF program: " ++ s)%bs, "")
       | compM.Ret e =>
           let (_, ctag, itag, ftag, cenv, fenv, nenv, _, log) := c_data' in
-          let s := cps_show.show_cenv cenv tt in              
-        (Ret (prims, cenv, ctag, itag, nenv, fenv, M.empty _, e), s)
+          let s := cps_show.show_cenv cenv tt in
+          let s_prims := M.fold1 (fun a '(k, _, _, _) => (a ++ ", " ++ (string_of_kername k))%bs) (snd prims) ""%bs in
+                                                                      
+        (Ret (prims, cenv, ctag, itag, nenv, fenv, M.empty _, e), (s ++ s_prims)%bs)
       end%positive.
     
   End Pipeline.
